LeanColls/FoldableOps.lean
@@ -8,25 +8,25 @@ import LeanColls.Classes
 
 namespace LeanColls
 
-class FoldableOps (C τ) [Foldable C τ] [BEq τ] where
+class FoldableOps (C τ) [Foldable C τ] where
   toList : C → List τ
-  h_toList : toList = Foldable.fold (· :: ·) []
   all : C → (τ → Bool) → Bool
-  h_all : all = List.all ∘ toList
-  contains : C → τ → Bool
-  h_contains : contains = List.contains ∘ toList
-
-instance [Foldable C τ] [BEq τ] : Inhabited (FoldableOps C τ) where
-  default := {
-    toList := _
-    h_toList := rfl
-    all := _
-    h_all := rfl
-    contains := _
-    h_contains := rfl
-  }
 
 namespace FoldableOps
+
+def defaultImpl (F : Foldable C τ) : FoldableOps C τ where
+  toList    := λ c    => Foldable.fold (fun acc x => x::acc) [] c |>.reverse
+  all       := λ c f  => Foldable.fold (fun acc x => acc && f x) true c
+
+instance [F : Foldable C τ] : Inhabited (FoldableOps C τ) where
+  default := defaultImpl F
+
+/- TODO: figure out how to generate foldable' generically
+def foldable' [F : Foldable C τ] [B : BEq τ] [M : Membership τ C]
+  (h_mem : ∀ c x, x ∈ c ↔ (defaultImpl F B).contains c x)
+  : Foldable' C τ M where
+  fold' := F.fold
+  -/
 
 theorem toList_ind [Foldable C τ] [BEq τ] [FoldableOps C τ] {α : Type u} {motive : List τ → Sort v}
         (nil : motive List.nil)
@@ -38,5 +38,16 @@ theorem toList_ind [Foldable C τ] [BEq τ] [FoldableOps C τ] {α : Type u} {mo
   exact cons _ _ (by assumption)
 
 end FoldableOps
+
+class FoldableEqOps (C τ) [Foldable C τ] [BEq τ] extends FoldableOps C τ where
+  contains : C → τ → Bool
+
+namespace FoldableEqOps
+
+def defaultImpl (F : Foldable C τ) (B : BEq τ) : FoldableEqOps C τ :=
+  { FoldableOps.defaultImpl F with
+    contains := λ c x  => Foldable.fold (fun acc y => acc || BEq.beq x y) true c}
+
+end FoldableEqOps
 
 end LeanColls
