LeanColls/Range.lean
@@ -1,32 +1,211 @@
+/-
+Copyright (c) 2022 James Gallicchio.
+
+Authors: James Gallicchio
+-/
+
 import LeanColls.List
 import LeanColls.AuxLemmas
 
 namespace LeanColls
 
-structure Range (n : Nat)
+/-! # Range
+
+Represents the first `n` natural numbers, e.g. [0, n).
+-/
+structure Range where
+  n : Nat
 
 namespace Range
 
-def fold : (Fin n → β → β) → β → Range n → β :=
-  let rec @[inline] loop {m α} (f : Fin m → α → α) acc i : α :=
-    if h:i < m then
-      loop f (f ⟨i,h⟩ acc) (i+1)
+def fold : (β → Nat → β) → β → Range → β :=
+  let rec @[inline] loop {α} (stop) (f : α → Nat → α) acc i : α :=
+    if h:i < stop then
+      loop stop f (f acc i) (i+1)
     else
       acc
-  λ f acc ⟨⟩ => loop f acc 0
-  termination_by loop _ _ i => m - i
+  λ f acc ⟨n⟩ =>
+    loop n f acc 0
+  termination_by loop i => stop - i
 
-theorem fold_ind {f : Fin n → β → β} {acc : β} {motive : Nat → β → Prop}
-  (init : motive 0 acc)
-  (step : ∀ i acc, (h : i < n) → motive i acc → motive i.succ (f ⟨i,h⟩ acc))
-  : motive n (fold f acc ⟨⟩)
+instance : Membership Nat Range where
+  mem x r := x < r.n
+
+def fold' : (r : Range) → (β → (i : Nat) → i ∈ r → β) → β → β :=
+  let rec @[inline] loop {α} (stop)
+    (f : α → (i : Nat) → i ∈ (⟨stop⟩ : Range) → α) acc i : α :=
+    if h:i < stop then
+      have : stop - (i + 1) < stop - i := by
+        rw [Nat.sub_dist]
+        apply Nat.sub_lt
+        exact Nat.zero_lt_sub_of_lt h
+        decide
+      have : i ∈ (⟨stop⟩ : Range) := h
+      loop stop f (f acc i this) (i+1)
+    else
+      acc
+  λ ⟨n⟩ f acc =>
+    loop n f acc 0
+  termination_by loop _ _ i => stop - i
+
+theorem fold_eq_fold' (n) (f : β → Nat → β) (acc : β)
+  : fold f acc ⟨n⟩ = fold' ⟨n⟩ (fun acc x _ => f acc x) acc
+  := by
+    simp [fold, fold']
+    suffices ∀ i, i ≤ n → fold.loop _ _ _ (n - i) = fold'.loop _ _ _ (n - i) by
+      have := this n
+      simp at this
+      exact this
+    intro i h_i
+    induction i generalizing acc with
+    | zero =>
+      unfold fold.loop
+      unfold fold'.loop
+      simp
+    | succ i ih =>
+      unfold fold.loop
+      unfold fold'.loop
+      split
+      case inr => trivial
+      case inl h =>
+      have : (n - Nat.succ i) + 1 = n - i := by
+        rw [Nat.succ_eq_add_one, Nat.sub_dist, Nat.sub_add_cancel _]
+        apply Nat.le_sub_of_add_le
+        rw [Nat.add_comm, ← Nat.succ_eq_add_one]
+        exact h_i
+      simp
+      rw [this, ih]
+      exact Nat.le_of_lt h_i
+
+theorem fold'_ind {stop : Nat}
+  {f : β → (i : Nat) → i ∈ (⟨stop⟩ : Range) → β}
+  {acc : β} {motive : (i : Nat) → i ≤ stop → β → Prop}
+  (base : motive 0 (Nat.zero_le _) acc)
+  (ind_step : ∀ i acc, (h : i < stop) →
+      motive i (Nat.le_of_lt h) acc → motive (i+1) h (f acc i h))
+  : motive stop (Nat.le_refl _) (fold' (⟨stop⟩ : Range) f acc)
+  :=
+  let rec loop i (acc : β) (h_i : i ≤ stop) (h_acc : motive i h_i acc)
+    : motive stop (Nat.le_refl _) (fold'.loop stop f acc i) :=
+    if h:i < stop then by
+      unfold fold'.loop
+      simp [h]
+      exact loop (i+1) (f acc i h) h (ind_step i acc h h_acc)
+    else by
+      have : i = stop := (Nat.eq_or_lt_of_le h_i).elim (id) (False.elim ∘ h)
+      unfold fold'.loop
+      simp [h]
+      cases this
+      exact h_acc
+  loop 0 acc (Nat.zero_le _) base
+  termination_by loop _ _ _i => stop - i
+
+theorem fold_ind {stop : Nat}
+  {f : β → Nat → β}
+  {acc : β} {motive : (i : Nat) → i ≤ stop → β → Prop}
+  (base : motive 0 (Nat.zero_le _) acc)
+  (ind_step : ∀ i acc, (h : i < stop) →
+      motive i (Nat.le_of_lt h) acc → motive (i+1) h (f acc i))
+  : motive stop (Nat.le_refl _) (fold f acc (⟨stop⟩ : Range))
+  := by
+  rw [fold_eq_fold']
+  apply fold'_ind <;> assumption
+
+instance : Foldable Range Nat where
+  fold := fold 
+
+instance : FoldableOps Range Nat := default
+
+instance : Foldable' Range Nat inferInstance where
+  fold' := fold'
+
+instance : Iterable Range Nat where
+  ρ := Nat × Nat
+  step := λ (i,stop) => if h:i < stop then some (i, (i.succ, stop)) else none
+  toIterator := λ r => (0,r.n)
+
+end Range
+
+/-! # Range.Complex
+
+A more complicated range, defined by a `start`, `step`, and `stop` value.
+
+The sequence proceeds: `start`, `start + step`, `start + 2 * step`, ...
+
+... until the value passes `stop`. For `step > 0`, the values are upper bounded
+by `stop`, while for `step < 0` the values are lower bounded by `stop`.
+
+Similar to `Std.Range`, but allows negative values for start/stop/step.
+-/
+structure Range.Complex where
+  start : Int
+  stop : Int
+  step : Int
+  h_step : step ≠ 0
+
+namespace Range.Complex
+
+/-
+def fold : (β → Int → β) → β → Range.Complex → β :=
+  let rec @[inline] loop {α} (start stop step h_step) (f : α → Int → α) acc i : α :=
+    if h:i < stop then
+      have : stop - (i + step) < stop - i := by
+        rw [Int.]
+        apply Nat.sub_lt
+        exact Nat.zero_lt_sub_of_lt h
+        exact h_step
+      loop start stop step h_step f (f acc i) (i+step)
+    else
+      acc
+  λ f acc ⟨start,stop,step, h_step⟩ =>
+    if h:step > 0 then loop start stop step h_step f acc 0 else acc
+  termination_by loop _ _ i => stop - i
+
+instance : Membership Nat Range where
+  mem x r := x < r.stop ∧ ∃ k, x = r.start + k * r.step
+
+def fold' : (r : Range) → (β → (i : Nat) → i ∈ r → β) → β → β :=
+  let rec @[inline] loop {α} (start stop step h_step)
+    (f : α → (i : Nat) → i ∈ (⟨start,stop,step,h_step⟩ : Range) → α) acc
+    i (h_i : ∃ k, i = start + k * step) : α :=
+    if h:i < stop then
+      have : stop - (i + step) < stop - i := by
+        rw [Nat.sub_dist]
+        apply Nat.sub_lt
+        exact Nat.zero_lt_sub_of_lt h
+        assumption
+      have : i ∈ (⟨start,stop,step,h_step⟩ : Range) := ⟨h_step, h, h_i⟩
+      loop start stop step h_step f (f acc i this) (i+step) (by
+        cases h_i; case intro k h_i =>
+        apply Exists.intro (k+1)
+        simp [Nat.succ_mul]
+        rw [←Nat.add_assoc, h_i]
+      )
+    else
+      acc
+  λ ⟨start,stop,step,h_step⟩ f acc =>
+    loop start stop step h_step f acc start ⟨0,by simp⟩
+  termination_by loop _ _ i _ => stop - i
+
+def last (r : Range) := r.start + ((r.stop - r.start) / r.step) * r.step
+
+theorem mem_last (r : Range) : r.last ∈ r := by
+  simp [last, Membership.mem]
+  sorry
+
+theorem fold_ind {start stop step : Nat}
+  {f : β → (i : Nat) → i ∈ (⟨start,stop,step⟩ : Range) → β}
+  {acc : β} {motive : Nat → β → Prop}
+  (base : motive 0 acc)
+  (ind_step : ∀ i acc, (h : i ∈ (⟨start,stop,step⟩ : Range)) → motive i acc → motive (i+step) (f acc i h))
+  : motive n (fold' (⟨start,stop,step⟩ : Range) f acc)
   :=
   let rec loop i (acc : β) (h_i : i ≤ n) (h_acc : motive i acc)
-    : motive n (fold.loop f acc i) :=
+    : motive i () :=
     if h:i < n then by
       unfold fold.loop
       simp [h]
-      exact loop i.succ (f ⟨i,h⟩ acc) h (step i acc h h_acc)
+      exact loop i.succ (f acc ⟨i,h⟩) h (step i acc h h_acc)
     else by
       have : i = n := (Nat.eq_or_lt_of_le h_i).elim (id) (False.elim ∘ h)
       unfold fold.loop
@@ -37,24 +216,20 @@ theorem fold_ind {f : Fin n → β → β} {acc : β} {motive : Nat → β → P
   termination_by loop _ _ _i => n - i
 
 
-instance : Foldable (Range n) (Fin n) where
-  fold := fold
+instance : Foldable Range Nat where
+  fold := fold 
 
-instance : Iterable (Range n) (Fin n) where
+instance : FoldableOps Range Nat := default
+
+instance : Foldable' Range Nat inferInstance where
+  fold' := fold'
+
+instance : Iterable Range Nat where
   ρ := Nat
   step := λ i => if h:i < n then some ⟨⟨i,h⟩,i.succ⟩ else none
   toIterator := λ _ => 0
+-/
 
-def toList (r : Range n) : List (Fin n) := Unfoldable.unfold r
-
-instance : FoldableOps (Range n) (Fin n) where
-  toList := toList
-  h_toList := by sorry
-  all := _
-  h_all := by rfl
-  contains _ i := i < n
-  h_contains := by sorry
-
-end Range
+end Range.Complex
 
 end LeanColls
