LeanColls/View.lean
@@ -1,47 +1,61 @@
 /-
 Copyright (c) 2022 James Gallicchio.
 
-Authors: James Gallicchio, Mario Carneiro
+Authors: James Gallicchio
 -/
 
 import LeanColls.Classes
+import LeanColls.FoldableOps
 
 namespace LeanColls
 
-inductive View : Type u → Type (u+1)
-| of {F τ} (c : F) [Foldable F τ] : View τ
-| map (f : τ → τ') (v : View τ) : View τ'
-| filter (f : τ → Bool) (v : View τ) : View τ
-| filterMap (f : τ → Option τ') (v : View τ) : View τ'
+structure View (τ) where
+  fold : {β : Type w} → (β → τ → β) → β → β
 
 namespace View
 
+instance : Foldable (View τ) τ where
+  fold f acc c := c.fold f acc
+
+instance [BEq τ] : FoldableOps (View τ) τ := default
+
 @[inline]
-def fold (foldF : τ → β → β) (foldAcc : β) : View τ → β
-| of c          => Foldable.fold foldF foldAcc c
-| map f v       => fold (foldF ∘ f) foldAcc v
-| filter f v    =>
-    fold (λ x a =>
-      if f x then foldF x a else a
-    ) foldAcc v
-| filterMap f v =>
-    fold (λ x a =>
+def view {F τ} (c : F) [Foldable F τ] : View τ where
+  fold f acc := Foldable.fold f acc c
+
+@[inline]
+def map {τ : Type u} {τ' : Type v} (f : τ → τ') (v : View τ) : View τ' where
+  fold foldF foldAcc :=
+    v.fold (λ acc t => foldF acc (f t)) foldAcc
+
+@[inline]
+def filter (f : τ → Bool) (v : View τ) : View τ where
+  fold foldF foldAcc :=
+    v.fold (λ a x =>
+      if f x then foldF a x else a
+    ) foldAcc
+
+@[inline]
+def filterMap (f : τ → Option τ') (v : View τ) : View τ' where
+  fold := λ foldF foldAcc =>
+    v.fold (λ a x =>
       match f x with
       | none    => a
-      | some x' => foldF x' a
-    ) foldAcc v
+      | some x' => foldF a x'
+    ) foldAcc
 
-instance : Foldable (View τ) τ where
-  fold := fold
+instance : FoldableOps (View τ) τ := default
 
-/- Defines toList on a view by accumulating continuations
-May be more inefficient than building list in reverse +
-explicitly reversing it.
--/
-def toList (v : View τ) : List τ :=
-  v.fold (fun x k tl => k (x :: tl)) id
-  <| []
+structure WithMem (τ) (c : C) (M : outParam (Membership τ C)) where
+  fold' : {β : Type w} → (β → (x : τ) → x ∈ c → β) → β → β
 
-end View
+@[inline]
+def view' [Foldable' C τ M] (c : C) : WithMem τ c M where
+  fold' := Foldable'.fold' c
 
-end LeanColls
+namespace WithMem
+
+@[inline]
+def map' {τ : Type u} {c : C} {M} (v : View.WithMem τ c M) {τ' : Type v} (f : (x : τ) → M.mem x c → τ') : View τ' where
+  fold foldF foldAcc :=
+    v.fold' (λ acc t h => foldF acc (f t h)) foldAcc
