LeanColls/IndexedOps.lean
@@ -6,29 +6,39 @@ Authors: James Gallicchio
 
 import LeanColls.Classes
 import LeanColls.Range
+import LeanColls.View
 
 namespace LeanColls
 
+namespace IndexedOps
+
 instance [Indexed C τ] : Foldable C τ where
-  fold f init c := Range.fold (λ i acc => f (Indexed.nth c i) acc) init ⟨⟩
+  fold f init c :=
+    Range.fold' ⟨Size.size c⟩ (λ acc i h =>
+      f acc (Indexed.nth c ⟨i,h⟩)
+    ) init
 
 structure Slice (C) (τ : outParam (Type u)) [Indexed C τ] where
   c : C
   off : Nat
   len : Nat
-  h_range : off + len ≤ Indexed.size c
+  h_range : off + len ≤ Size.size c
 
 instance [Indexed C τ] : Indexed (Slice C τ) τ where
   size S := S.len
   nth S (i : Fin S.len) := Indexed.nth S.c ⟨S.off + i, Nat.le_trans (Nat.add_lt_add_left i.isLt _) (Slice.h_range S)⟩
 
 def IndexedEq [DecidableEq τ] [Indexed C₁ τ] [Indexed C₂ τ] (c₁ : C₁) (c₂ : C₂)
-  {h : Indexed.size c₁ = Indexed.size c₂} : Prop :=
+  {h : Size.size c₁ = Size.size c₂} : Prop :=
   ∀ i, Indexed.nth c₁ i = Indexed.nth c₂ ⟨i.val, by rw [←h]; exact i.isLt⟩
 
-class IndexedOps (C) (τ : outParam (Type u)) where
-  slice [Indexed C τ] (off len : Nat) (c : C)
-    {h : off + len ≤ Indexed.size c} : Slice C τ
+end IndexedOps
+
+class IndexedOps (C τ) [Indexed C τ] where
+  slice (off len : Nat) (c : C)
+    {h : off + len ≤ Size.size c} : IndexedOps.Slice C τ
+
+namespace IndexedOps
 
 instance [Indexed C τ] : Inhabited (IndexedOps C τ) where
   default := {
@@ -36,9 +46,15 @@ instance [Indexed C τ] : Inhabited (IndexedOps C τ) where
   }
 
 instance [Indexed C τ] : MapLike C Nat τ where
-  κ c := Range (Indexed.size c)
-  κ_hasMem c := ⟨λ i _ => i < Indexed.size c⟩
-  keySet c := @Range.mk (Indexed.size c)
-  get c i := Indexed.nth c ⟨i.val, i.property⟩
+  fold f acc c :=
+    Range.fold' ⟨Size.size c⟩ (λ acc i h_i =>
+      f acc (i, Indexed.nth c ⟨i,h_i⟩)
+    ) acc
+  get? c i :=
+    if h : i < Size.size c then
+      some (Indexed.nth c ⟨i, h⟩)
+    else none
+
+end IndexedOps
 
 end LeanColls
